Ground_PDDL_Exec_Imp/Ground_PDDL_NTA_Reduction_Impl.thy
@@ -1,5 +1,6 @@
 theory Ground_PDDL_NTA_Reduction_Impl
   imports Ground_PDDL_NTA_Reduction_Correctness
+    "Temporal_Planning.Temporal_PDDL_Checker_Explicit"
 begin
 
 
