Temporal_Planning_Common/TP_Utils.thy
@@ -1,4 +1,4 @@
-theory Utils
+theory TP_Utils
   imports Main "Containers.Containers"
 begin
 
